proof/correctness/Correctness_XMSS.ec
@@ -3,15 +3,90 @@ pragma Goals : printall.
 require import AllCore List RealExp IntDiv.
 from Jasmin require import JModel JArray.
 
-require import Params Parameters Address Notation Primitives Wots XMSS_MT_PRF.
+require import Types Params Parameters Address Notation Hash Primitives Wots XMSS_MT_PRF.
 require import XMSS_IMPL.
+require import Repr. 
+require import Array8 Array32 Array64 Array2144.
 
-require import Array8 Array32 Array64.
+(*---*) import NBytes.
 
-(*** Randomized Hashing ***)
-lemma thash_correct (_in : W8.t Array64.t,
-                     _pub_seed : W8.t Array32.t, 
-                     _addr:W32.t Array8.t) :
-    equiv[M_Hop1(Syscall).__thash_h ~ RandHash.rand_hash : true ==> true].
+require import Correctness_Mem Correctness_Hash.
+require import Utils.
+
+require import BitEncoding.
+(*---*) import BitChunking.
+
+(*** L Tree ***)
+
+lemma ltree_correct (_pk : W8.t Array2144.t, _pub_seed : W8.t Array32.t, _addr : W32.t Array8.t) : 
+    len = XMSS_WOTS_LEN /\ 
+    n = XMSS_N =>
+    equiv [
+      M(Syscall).__l_tree ~ LTree.ltree :
+      arg{1}.`2 = _pk /\
+      arg{1}.`3 = _pub_seed /\
+      arg{1}.`4 = _addr /\
+      arg{2} = (EncodeWotsPk _pk, _addr, to_list _pub_seed)
+      ==>
+      to_list res{1}.`1 = res{2}.`1 /\ (* wots pk *)
+      res{1}.`3 = res{2}.`2 (* address *)
+    ].
+proof.
+move => [#] *.
+proc. 
+auto => />.
+seq 3 1 : (#pre); first by auto. 
+seq 1 1 : (#pre /\ _len{2} = to_uint l{1} /\ _len{2} = 67);  first by auto.
+seq 2 1 : (
+  addr{1} = address{2} /\
+  pk{2} = EncodeWotsPk wots_pk{1} /\
+  _seed{2} = to_list pub_seed{1} /\
+  _len{2} = to_uint l{1} /\
+  _len{2} = 67
+); first by inline {1}; auto. 
+seq 1 1 : (
+  addr{1} = address{2} /\ 
+  (forall (k : int), 0 <= k < 32 => wots_pk{1}.[k] = nth witness (nth witness pk{2} 0) k) /\
+  size pk{2} = len /\
+  forall (t : W8.t list), t \in pk{2} => size t = n
+); last first.
+    + ecall {1} (_x_memcpy_u8u8_post tmp{1}).
+      auto => /> &1 &2 ???.
+      apply (eq_from_nth witness); [ rewrite (size_nth pk{2} 32 0);1,2:smt(); by rewrite size_to_list | smt(@Array32) ].
+(*-------------------------------------------------------------------------------------------------------------------------------------------*)
+while (
+  0 <= _len{2} <= 67 /\
+  _len{2} = to_uint l{1} /\
+  _seed{2} = to_list pub_seed{1} /\
+  size pk{2} = len /\
+  addr{1} = address{2} /\ 
+  (forall (k : int), 0 <= k < 32 => wots_pk{1}.[k] = nth witness (nth witness pk{2} 0) k) /\
+  (forall (t : W8.t list), t \in (pk{2}) => size t = n)
+); last by admit.
+
+    + seq 2 0 : (#pre /\ to_uint parent_nodes{1} = floor (len%r / 2%r)). 
+      * auto => /> &1 &2 *. 
+        have ->: truncateu8 (W256.one `&` (of_int 63)%W256) = W8.one by admit.
+        rewrite shr_div.
+        have ->: 2 ^ (to_uint W8.one %% 64) = 2 by smt(@W8).
+        admit.
+    
+     
+
+(* ------------------------- *)
+
+    + skip => /> &1 *. do split.
+
+smt().
+smt().
+rewrite size_enc_wots_pk /#.
+move => k ? ?. 
+    + admit. (* rewrite -nth_flatten. rewrite size_enc_wots_pk /#. rewrite (size_nth (EncodeWotsPk wots_pk{1}) 32 0); smt(size_enc_wots_pk ssize_enc_wots_pk). *)      
+smt(ssize_enc_wots_pk).
+smt(@W64 pow2_64).
+smt(@W64 pow2_64).
+qed.
+
+(*** Treehash ***)
 
 (******* exported functions ********)
